Plfl/StrongNorm.lean
@@ -1,0 +1,80 @@
+/-
+  Strong Normalization of Simply Typed Lambda Calculus
+-/
+
+import Plfl.STLC
+
+-- Trivial fact
+theorem value_halts : ∀ v, Val v → v ⇓ := by
+  intros v h
+  simp [halts]
+  apply Exists.intro v
+  apply And.intro Steps.refl h
+
+/-
+-- Does not work: It violates the strict positivity requirement for inductive definitions.
+inductive SN : Ty → Tm → Prop
+  | bool {e} : ∅ ⊢ e ∶ bool → e ⇓ → SN bool t
+  | arrow {τ₁ τ₂ e} : ∅ ⊢ e ∶ τ₁ ⇒ τ₂ → e ⇓ → (∀ e', SN τ₁ e' → SN τ₂ (e ⬝ e')) → SN (τ₁ ⇒ τ₂) e
+-/
+
+def SN : Ty → Tm → Prop
+  | .bool, e => (∀ {Γ}, Γ ⊢ e ∶ bool) ∧ e ⇓
+  | .arr τ₁ τ₂, e => (∀ {Γ}, Γ ⊢ e ∶ τ₁ ⇒ τ₂) ∧ e ⇓ ∧ ∀ e', SN τ₁ e' → SN τ₂ (e ⬝ e')
+
+abbrev Substs := List (String × Tm)
+
+-- Multi substitution
+def msubst (γ : Substs) (e : Tm) : Tm :=
+  match γ with
+  | .nil => e
+  | (x, s) :: γ' => msubst γ' ([x ↦ s] e)
+
+notation γ "⟦" e "⟧" => msubst γ e
+
+def Substs.dom (γ : Substs) : List String :=
+  γ.map Prod.fst
+
+def Context.dom (Γ : Context) : List String :=
+  match Γ with
+  | Context.empty => []
+  | Γ' ; x : _ => x :: Γ'.dom
+
+def substs_satisfies_context (γ : Substs) (Γ : Context) : Prop :=
+  γ.dom = Γ.dom ∧ ∀ x τ, Γ ∋ x : τ → SN τ (γ ⟦ %x ⟧)
+
+infix:50 " ⊨ " => substs_satisfies_context
+
+theorem empty_substs_satisfies_empty_context : [] ⊨ ∅ := by
+  simp [substs_satisfies_context]
+  apply And.intro rfl
+  intros x τ h
+  cases h
+
+theorem msubst_preserves_typing {Γ e τ γ} : Γ ⊢ e ∶ τ → γ ⊨ Γ → ∅ ⊢ γ ⟦ e ⟧ ∶ τ := by
+  intro h h'
+  sorry
+
+theorem sn_preserves_by_reduction {e τ} : ∅  ⊢ e ∶ τ → e ——→ e' → (SN τ e ↔ SN τ e') := by
+  intros h h'
+  apply Iff.intro
+  intro hsn
+  sorry
+
+theorem sn_membership_with_subst {Γ e τ γ} : γ ⊨ Γ → Γ ⊢ e ∶ τ → SN τ (γ ⟦ e ⟧) := by
+  intros h h'
+  induction h' generalizing γ
+  case tru =>
+  sorry
+
+theorem sn_membership {e τ} : ∅ ⊢ e ∶ τ → SN τ e :=
+  sn_membership_with_subst empty_substs_satisfies_empty_context
+
+theorem sn_member_is_normalizing {e τ} : SN τ e → e ⇓ := by
+  intro h
+  induction τ
+  . apply h.2
+  . apply h.2.1
+
+theorem strong_normalization : ∀ {e τ}, ∅ ⊢ e ∶ τ → e ⇓ :=
+  λ h => sn_member_is_normalizing (sn_membership h)
