lakefile.lean
@@ -3,13 +3,9 @@ open Lake DSL
 
 package «plfl» where
   -- add package configuration options here
-  moreLinkArgs := #["-L./.lake/packages/LeanCopilot/.lake/build/lib", "-lctranslate2"]
 
 require mathlib from git
   "https://github.com/leanprover-community/mathlib4.git"
-
-require LeanCopilot from git
-  "https://github.com/lean-dojo/LeanCopilot.git" @ "v1.0.0"
 
 lean_lib «Plfl» where
   -- add library configuration options here
